Thesis/TwoLabel.lean
@@ -6,33 +6,35 @@ namespace Componentwise
 
 -- We can reuse the notions of main road and rewrite distance from
 -- the proof of proposition 14.2.30.
-open MainRoad RewriteDistance
+open RewriteDistance
 
 open Relation
 
 variable
   {α I: Type} {A: ARS α I}
-  (C: Component A)
+  {C: Component A}
   (hcp: cofinality_property_conv A)
+
+variable
+  {N: ℕ∞} {f: ℕ → C.Subtype}
+  (main_road: reduction_seq C.ars.union_rel N f)
+  {hacyclic: main_road.acyclic}
+  (hcr: cofinal_reduction main_road)
+
 
 -- At some points we will require there to be a well-order on α.
 -- Note that this can always be satisfied, by the well-ordering theorem
 -- (see `exists_wellOrder`).
 variable [LinearOrder α]
 
-def step_on_main_road (a b: C.Subtype) :=
-  ∃n, a = ((main_road_f C hcp) n) ∧
-      b = ((main_road_f C hcp) (n + 1)) ∧
-      n < (main_road_len C hcp)
-
-def on_main_road_imp_d0 {a} (heq: a ∈ (main_road C hcp).elems):
-    (dX a (main_road C hcp).elems (main_road_cr C hcp a)).val = 0 := by
+def on_main_road_imp_d0 {a} (heq: a ∈ main_road.elems):
+    (dX a main_road.elems (hcr a)).val = 0 := by
   have: is_reduction_seq_from C.ars.union_rel a a (fun n ↦ a) 0 := by
     simp
     exact reduction_seq.refl C.ars.union_rel fun n ↦ a
 
   by_contra h
-  have hzerolt: 0 < (dX a (main_road C hcp).elems (main_road_cr C hcp a)).val := by
+  have hzerolt: 0 < (dX a main_road.elems (hcr a)).val := by
     omega
 
   simp at heq
@@ -43,26 +45,22 @@ def on_main_road_imp_d0 {a} (heq: a ∈ (main_road C hcp).elems):
   use a
   rw [<-heq]
   constructor
-  · simp [main_road_f]
+  · simp
     use n
   · rw [<-heq] at this
     exact this
 
 
-def step_on_main_road_imp_step {a b: C.Subtype} (hs: step_on_main_road C hcp a b): C.ars.union_rel a b := by
-  simp [step_on_main_road] at hs
-  obtain ⟨n, heq₁, heq₂, hlt⟩ := hs
-  have := (main_road C hcp) n hlt
-  rw [heq₁, heq₂]
-  assumption
+def step_on_main_road_imp_step {a b: C.Subtype} (hs: main_road.contains a b): C.ars.union_rel a b := by
+  simp [reduction_seq.contains] at hs
+  obtain ⟨n, rfl, rfl, hlt⟩ := hs
+  exact main_road n hlt
 
 def step_minimizing (a b: C.Subtype) :=
-  let mr := main_road C hcp;
-  let hcr := main_road_cr C hcp;
-  C.ars.union_rel a b ∧ (dX a mr.elems (hcr a)).val = (dX b mr.elems (hcr b)).val + 1 ∧ -- a -> b ∧ d(a) = d(b) + 1
-  ∀b', C.ars.union_rel a b' ∧ (dX b mr.elems (hcr b)).val = (dX b' mr.elems (hcr b')).val → b' ≥ b -- for all b' s.t. a -> b' ∧ d(b) = d(b'), b' ≥ b.
+  C.ars.union_rel a b ∧ (dX a main_road.elems (hcr a)).val = (dX b main_road.elems (hcr b)).val + 1 ∧ -- a -> b ∧ d(a) = d(b) + 1
+  ∀b', C.ars.union_rel a b' ∧ (dX b main_road.elems (hcr b)).val = (dX b' main_road.elems (hcr b')).val → b' ≥ b -- for all b' s.t. a -> b' ∧ d(b) = d(b'), b' ≥ b.
 
-def step_minimizing_imp_step {a b: C.Subtype} (hs: step_minimizing C hcp a b):
+def step_minimizing_imp_step {a b: C.Subtype} (hs: step_minimizing main_road hcr a b):
     C.ars.union_rel a b := by
   simp [step_minimizing] at hs
   tauto
@@ -70,37 +68,39 @@ def step_minimizing_imp_step {a b: C.Subtype} (hs: step_minimizing C hcp a b):
 def C': ARS C.Subtype (Fin 2) where
   rel := fun n b c ↦
     match n with
-      | 0 => (step_on_main_road C hcp b c ∨ step_minimizing C hcp b c)
-      | 1 => C.ars.union_rel b c ∧ ¬(step_on_main_road C hcp b c ∨ step_minimizing C hcp b c)
+      | 0 => (main_road.contains b c ∨ step_minimizing main_road hcr b c)
+      | 1 => C.ars.union_rel b c ∧ ¬(main_road.contains b c ∨ step_minimizing main_road hcr b c)
 
 
 /-- Lemma 4.9(i): our labeled ARS is reduction-equivalent to C.ars. -/
 lemma C'.reduction_equivalent (b c: C.Subtype):
-    C.ars.union_rel b c ↔ (C' C hcp).union_rel b c := by
+    C.ars.union_rel b c ↔ (C' main_road hcr).union_rel b c := by
   constructor <;> intro h
   · simp only [C', ARS.union_rel]
-    by_cases h: (step_on_main_road C hcp b c ∨ step_minimizing C hcp b c)
+    by_cases h: (main_road.contains b c ∨ step_minimizing main_road hcr b c)
     · use 0
     · use 1
   · simp [C', ARS.union_rel] at h
     obtain ⟨i, hi⟩ := h
     split at hi
-    · cases hi <;> simp [step_on_main_road_imp_step, step_minimizing_imp_step, *]
+    · cases hi
+      · simp [step_on_main_road_imp_step main_road, *]
+      · simp [step_minimizing_imp_step main_road, *]
     · simpa [ARS.union_rel] using hi.left
 
 /-- Equivalent to steps_along_hseq in Prop 14.2.30. -/
-lemma steps_on_main_road {n k: ℕ} (hk: n + k < (main_road_len C hcp) + 1):
-    ((C' C hcp).rel 0)∗ (main_road_f C hcp n) (main_road_f C hcp (n + k)) := by
+lemma steps_on_main_road {n k: ℕ} (hk: n + k < N + 1):
+    ((C' main_road hcr).rel 0)∗ (f n) (f (n + k)) := by
   induction k generalizing n with
   | zero => rfl
   | succ k ih =>
-    have hlt: n + k < (main_road_len C hcp) := by
-      cases h: (main_road_len C hcp)
+    have hlt: n + k < N := by
+      cases h: N
       · norm_cast; exact WithTop.coe_lt_top _
       · rw [h] at hk
         norm_cast at hk ⊢
         omega
-    have hlt': n + k < (main_road_len C hcp) + 1 := lt_of_lt_of_le hlt le_self_add
+    have hlt': n + k < N + 1 := lt_of_lt_of_le hlt le_self_add
     apply ReflTransGen.tail (ih hlt')
 
     simp [C']
@@ -110,8 +110,8 @@ lemma steps_on_main_road {n k: ℕ} (hk: n + k < (main_road_len C hcp) + 1):
     norm_cast
 
 /-- Lemma 4.9(ii); if a, b ∈ M, ∃d, a ->>_0 d ∧ b ->>_0 d. -/
-lemma L4_9_ii (a b: C.Subtype) (ha: a ∈ (main_road C hcp).elems) (hb: b ∈ (main_road C hcp).elems):
-    ∃d, ((C' C hcp).rel 0)∗ a d ∧ ((C' C hcp).rel 0)∗ b d := by
+lemma L4_9_ii (a b: C.Subtype) (ha: a ∈ main_road.elems) (hb: b ∈ main_road.elems):
+    ∃d, ((C' main_road hcr).rel 0)∗ a d ∧ ((C' main_road hcr).rel 0)∗ b d := by
   simp at ha hb
 
   obtain ⟨n₁, hlt₁, heq₁⟩ := ha
@@ -132,59 +132,56 @@ lemma L4_9_ii (a b: C.Subtype) (ha: a ∈ (main_road C hcp).elems) (hb: b ∈ (m
     norm_cast
   · rfl
 
+include hacyclic in
 /-- There is at most one b s.t. a ->₀ b. -/
 lemma L4_9_iii {a b b': C.Subtype}:
-    (C' C hcp).rel 0 a b ∧ (C' C hcp).rel 0 a b' → b = b' := by
+    (C' main_road hcr).rel 0 a b ∧ (C' main_road hcr).rel 0 a b' → b = b' := by
   rintro ⟨hb, hb'⟩
-
-  have hacyclic := (main_road_acyclic C hcp)
 
   -- we distinguish between the case where a is on the main road, and the case
   -- where a is not on the main road.
-  by_cases h: ∃n, a = main_road_f C hcp n ∧ n < (main_road_len C hcp + 1)
-  · have hmem: a ∈ (main_road C hcp).elems := by
+  by_cases h: ∃n, a = f n ∧ n < N + 1
+  · have hmem: a ∈ main_road.elems := by
       obtain ⟨n, hn⟩ := h
       use n
-      simp [main_road_f, main_road_len] at hn ⊢
       tauto
 
-    have d0 := on_main_road_imp_d0 C hcp hmem
+    have d0 := on_main_road_imp_d0 main_road hcr hmem
     -- steps a->b and a->b' cannot be minimizing, as a = 0 and 0 cannot be n + 1.
-    replace hb: step_on_main_road C hcp a b := by
+    replace hb: main_road.contains a b := by
       apply hb.resolve_right
       rw [step_minimizing]
       omega
 
-    replace hb': step_on_main_road C hcp a b' := by
+    replace hb': main_road.contains a b' := by
       apply hb'.resolve_right
       rw [step_minimizing]
       omega
 
-    rw [step_on_main_road] at hb hb'
+    rw [reduction_seq.contains] at hb hb'
     obtain ⟨n, heqa₁, heqb, hlt₁⟩ := hb
     obtain ⟨n', heqa₂, heqb', hlt₂⟩ := hb'
 
-    rw [heqb', heqb]
+    rw [<-heqb', <-heqb]
     congr
     apply hacyclic hlt₁ hlt₂
-    simp [main_road_f] at heqa₁ heqa₂
-    rw [<-heqa₁, <-heqa₂]
-  · replace hb: step_minimizing C hcp a b := by
+    rw [heqa₁, heqa₂]
+  · replace hb: step_minimizing main_road hcr a b := by
       apply hb.resolve_left
       push_neg at h
       rintro ⟨n, hn⟩
-      specialize h n hn.left
+      specialize h n hn.left.symm
       apply not_le_of_gt hn.2.2
-      trans (main_road_len C hcp) + 1
+      trans N + 1
       · apply le_self_add
       · exact h
-    replace hb': step_minimizing C hcp a b' := by
+    replace hb': step_minimizing main_road hcr a b' := by
       apply hb'.resolve_left
       push_neg at h
       rintro ⟨n, hn⟩
-      specialize h n hn.left
+      specialize h n hn.left.symm
       apply not_le_of_gt hn.2.2
-      trans (main_road_len C hcp) + 1
+      trans N + 1
       · apply le_self_add
       · exact h
 
@@ -200,16 +197,16 @@ lemma L4_9_iii {a b b': C.Subtype}:
 
 variable [WellFoundedLT α]
 
-lemma L4_9_iv (a: C.Subtype) (ha: a ∉ (main_road C hcp).elems):
-    ∃b, (C' C hcp).rel 0 a b ∧
-      (dX a (main_road C hcp).elems (main_road_cr C hcp a)).val =
-      (dX b (main_road C hcp).elems (main_road_cr C hcp b)).val + 1 := by
-  obtain ⟨n, hdX⟩: ∃n, (dX a (main_road C hcp).elems (main_road_cr C hcp a)).val = n + 1 := by
-    suffices: (dX a (main_road C hcp).elems (main_road_cr C hcp a)).val ≠ 0
+lemma L4_9_iv (a: C.Subtype) (ha: a ∉ main_road.elems):
+    ∃b, (C' main_road hcr).rel 0 a b ∧
+      (dX a main_road.elems (hcr a)).val =
+      (dX b main_road.elems (hcr b)).val + 1 := by
+  obtain ⟨n, hdX⟩: ∃n, (dX a main_road.elems (hcr a)).val = n + 1 := by
+    suffices: (dX a main_road.elems (hcr a)).val ≠ 0
     · exact Nat.exists_eq_succ_of_ne_zero this
 
     intro hdx
-    have := dX.spec (main_road C hcp).elems (main_road_cr C hcp a)
+    have := dX.spec main_road.elems (hcr a)
     rw [hdx] at this
 
     obtain ⟨f, x, hxmem, hseq⟩ := this
@@ -222,20 +219,20 @@ lemma L4_9_iv (a: C.Subtype) (ha: a ∉ (main_road C hcp).elems):
     apply ha
     rw [heq, <-hseq.left, <-hseq.right.left]
 
-  obtain ⟨f, m, hmem, heq₁, heq₂, hseq⟩ := dX.spec (main_road C hcp).elems (main_road_cr C hcp a)
+  obtain ⟨f, m, hmem, heq₁, heq₂, hseq⟩ := dX.spec main_road.elems (hcr a)
   have hrel: C.ars.union_rel (f 0) (f 1) := by
     apply hdX ▸ hseq; norm_num
 
   rw [hdX]
 
-  have hdXb: dX (f 1) (main_road C hcp).elems (main_road_cr C hcp (f 1)) = n := by
+  have hdXb: dX (f 1) main_road.elems (hcr (f 1)) = n := by
     apply le_antisymm
-    · apply dX_step_le hcp a m hmem
+    · apply dX_step_le hcr a m hmem
       and_intros
       · exact heq₁
       · exact hdX ▸ heq₂
       · exact hdX ▸ hseq
-    · apply dX_step_ge hcp (f 0) (f 1)
+    · apply dX_step_ge hcr (f 0) (f 1)
       · exact hrel
       · exact heq₁ ▸ hdX
 
@@ -243,7 +240,7 @@ lemma L4_9_iv (a: C.Subtype) (ha: a ∉ (main_road C hcp).elems):
   -- now we need to pick the minimal one. Here we need the well-order on α,
   -- because we need the property that there is a minimal α for any set.
 
-  let B := { b' | C.ars.union_rel a b' ∧ (dX a (main_road C hcp).elems (main_road_cr C hcp a)).val = (dX b' (main_road C hcp).elems (main_road_cr C hcp b')).val + 1}
+  let B := { b' | C.ars.union_rel a b' ∧ (dX a main_road.elems (hcr a)).val = (dX b' main_road.elems (hcr b')).val + 1}
 
   have hnonempty: B.Nonempty := by
     use (f 1)
@@ -272,26 +269,26 @@ lemma L4_9_iv (a: C.Subtype) (ha: a ∉ (main_road C hcp).elems):
   · rw [<-hbmem.right, hdX]
 
 
-lemma L4_9_v (a: C.Subtype) (n: ℕ) (hn: n = dX a (main_road C hcp).elems (main_road_cr C hcp a)):
-    ∃m ∈ (main_road C hcp).elems, ((C' C hcp).rel 0)∗ a m := by
+lemma L4_9_v (a: C.Subtype) (n: ℕ) (hn: n = dX a main_road.elems (hcr a)):
+    ∃m ∈ main_road.elems, ((C' main_road hcr).rel 0)∗ a m := by
   induction n generalizing a with
   | zero =>
-    have := dX.spec (main_road C hcp).elems (main_road_cr C hcp a)
+    have := dX.spec main_road.elems (hcr a)
     rw [<-hn] at this
     obtain ⟨f, m, hmem, hseq⟩ := this
     use m, hmem
     unfold is_reduction_seq_from at hseq
     rw [<-hseq.1, <-hseq.2.1]
   | succ n ih =>
-    have := dX.spec (main_road C hcp).elems (main_road_cr C hcp a)
-    obtain ⟨f, m, hmem, hseq⟩ := this
+    have := dX.spec main_road.elems (hcr a)
+    obtain ⟨f', m, hmem, hseq⟩ := this
 
-    have ha: a ∉ (main_road C hcp).elems := by
+    have ha: a ∉ main_road.elems := by
       by_contra ha
-      have := on_main_road_imp_d0 _ hcp ha
+      have := on_main_road_imp_d0 _ hcr ha
       omega
 
-    obtain ⟨b, hbrel, hgt⟩ := L4_9_iv C hcp a ha
+    obtain ⟨b, hbrel, hgt⟩ := L4_9_iv main_road hcr a ha
 
     obtain ⟨m', hmem', hseq⟩ := ih b (by omega)
 
@@ -301,7 +298,8 @@ lemma L4_9_v (a: C.Subtype) (n: ℕ) (hn: n = dX a (main_road C hcp).elems (main
     exact hbrel
     exact hseq
 
-lemma C'.locally_decreasing: locally_decreasing (C' C hcp) := by
+include hacyclic in
+lemma C'.locally_decreasing: locally_decreasing (C' main_road hcr) := by
   rintro a b c i j ⟨hab, hac⟩
 
   by_cases heq: b = c
@@ -314,14 +312,15 @@ lemma C'.locally_decreasing: locally_decreasing (C' C hcp) := by
     by_contra!
     obtain ⟨rfl, rfl⟩: i = 0 ∧ j = 0 := by omega
     apply heq
-    apply L4_9_iii C hcp ⟨hab, hac⟩
+    apply L4_9_iii main_road hcr ⟨hab, hac⟩
+    assumption
 
-  obtain ⟨mb, hmbmem, hmbseq⟩ := L4_9_v C hcp b (dX b (main_road C hcp).elems (main_road_cr C hcp b)) rfl
-  obtain ⟨mc, hmcmem, hmcseq⟩ := L4_9_v C hcp c (dX c (main_road C hcp).elems (main_road_cr C hcp c)) rfl
+  obtain ⟨mb, hmbmem, hmbseq⟩ := L4_9_v main_road hcr b (dX b main_road.elems (hcr b)) rfl
+  obtain ⟨mc, hmcmem, hmcseq⟩ := L4_9_v main_road hcr c (dX c main_road.elems (hcr c)) rfl
 
-  obtain ⟨d, hd₁, hd₂⟩ := L4_9_ii C hcp mb mc hmbmem hmcmem
+  obtain ⟨d, hd₁, hd₂⟩ := L4_9_ii main_road hcr mb mc hmbmem hmcmem
 
-  have (a b: C.Subtype): (C' C hcp).rel 0 a b → ((C' C hcp).union_lt i ∪ (C' C hcp).union_lt j) a b := by
+  have (a b: C.Subtype): (C' main_road hcr).rel 0 a b → ((C' main_road hcr).union_lt i ∪ (C' main_road hcr).union_lt j) a b := by
     introv h
     rcases this with (rfl | rfl)
     · left
@@ -358,10 +357,11 @@ def dcr₂_component (hcp: cofinality_property A): ∀(C: Component A), DCRn 2 C
   unfold DCRn
   obtain ⟨linorder, wellfounded⟩ := exists_wellOrder α
 
-  use Componentwise.C' C hcp.to_conv
+  use Componentwise.C' (MainRoad.main_road C hcp.to_conv) (MainRoad.main_road_cr C hcp.to_conv)
   constructor
   · ext
     rw [<-Componentwise.C'.reduction_equivalent]
   · apply Componentwise.C'.locally_decreasing
+    exact MainRoad.main_road_acyclic C hcp.to_conv
 
 end Thesis.TwoLabel
